StructuredEncryption/src/AwsCryptographyStructuredEncryptionOperations.dfy
@@ -1,37 +1,33 @@
 // Copyright Amazon.com Inc. or its affiliates. All Rights Reserved.
 // SPDX-License-Identifier: Apache-2.0
 include "../Model/AwsCryptographyStructuredEncryptionTypes.dfy"
-include "../../private-aws-encryption-sdk-dafny-staging/AwsCryptographicMaterialProviders/test/TestUtils.dfy"
 include "Header.dfy"
+include "Paths.dfy"
+include "Crypt.dfy"
+include "Util.dfy"
 
 module AwsCryptographyStructuredEncryptionOperations refines AbstractAwsCryptographyStructuredEncryptionOperations {
+  import opened StructuredEncryptionUtil
+
   import Base64
   import CMP = AwsCryptographyMaterialProvidersTypes
+  import CSE = AwsCryptographyStructuredEncryptionTypes
+  import Prim = AwsCryptographyPrimitivesTypes
   import Random
   import Aws.Cryptography.Primitives
-  import Header
+  import Header = StructuredEncryptionHeader
   import MaterialProviders
-  import TestUtils
+  import Crypt = StructuredEncryptionCrypt
+  import Paths = StructuredEncryptionPaths
+  import Sets
+  import Digest
+  import Defaults
 
   datatype Config = Config(
     primatives : Primitives.AtomicPrimitivesClient
   )
 
   type InternalConfig = Config
-
-  // UTF-8 encoded "THIS_IS_NOT_ENCRYPTED"
-  // TODO this is temporary, only used for our "fake" encryption
-  // in order to make it clear that the value is not actually being encrypted yet.
-  const THIS_IS_NOT_ENCRYPTED: UTF8.ValidUTF8Bytes :=
-    var s := [0x54, 0x48, 0x49, 0x53, 0x5f, 0x49, 0x53, 0x5f, 0x4e, 0x4f, 0x54, 0x5f, 0x45, 0x4e, 0x43, 0x52, 0x59, 0x50, 0x54, 0x45, 0x44];
-    assert UTF8.ValidUTF8Range(s, 0, 21);
-    s
-
-  // TODO: This is temporary in order to support "fake" encryption with DDB,
-  // which is a placeholder to demonstrate the crypto schema is piping to this
-  // layer as expected when testing end to end with the DDB Encryption interceptor.
-  const DDB_STRING_TYPE_ID : seq<uint8> := [0x00, 0x01];
-  const BYTES_TYPE_ID : seq<uint8> := [0xFF, 0xFF];
 
   predicate ValidInternalConfig?(config: InternalConfig)
   {config.primatives.ValidState()}
@@ -48,6 +44,101 @@ module AwsCryptographyStructuredEncryptionOperations refines AbstractAwsCryptogr
     && (output.Success? && input.plaintextStructure.content.Terminal? ==> output.value.encryptedStructure.content.Terminal?)
   }
 
+  // given a list of CryptoSchema, return only the ones with an Action matching the supplied function
+  function method {:tailrecursion} {:opaque} FilterSchema(orig : seq<Bytes>, canonSchema : map<Bytes, CryptoSchema>, f : (CryptoAction) -> bool)
+    : (ret : seq<Bytes>)
+    requires forall k <- orig :: k in canonSchema && canonSchema[k].content.Action?
+    ensures forall k <- ret :: k in orig
+  {
+    if |orig| == 0 then
+      []
+    else if f(canonSchema[orig[0]].content.Action) then
+      [orig[0]] + FilterSchema(orig[1..], canonSchema, f)
+    else
+      FilterSchema(orig[1..], canonSchema, f)
+  }
+
+  // given a list of AuthenticateSchema, return only the ones with an Action matching the supplied value
+  function method {:tailrecursion} {:opaque} FilterAuth(orig : seq<Bytes>, canonSchema : map<Bytes, AuthenticateSchema>, action : AuthenticateAction)
+    : (ret : seq<Bytes>)
+    requires forall k <- orig :: k in canonSchema && canonSchema[k].content.Action?
+    ensures forall k <- ret :: k in orig
+  {
+    if |orig| == 0 then
+      []
+    else if canonSchema[orig[0]].content.Action == action then
+      [orig[0]] + FilterAuth(orig[1..], canonSchema, action)
+    else
+      FilterAuth(orig[1..], canonSchema, action)
+  }
+
+  // given a list of keys, return only those that should be encrypted, according to the legend
+  function method {:tailrecursion} {:opaque} FilterEncrypted(keys : seq<Bytes>, legend : Header.Legend)
+    : (ret : seq<Bytes>)
+    requires |keys| == |legend|
+    ensures forall k <- ret :: k in keys
+  {
+    if |keys| == 0 then
+      []
+    else if legend[0] == Header.ENCRYPT_AND_SIGN_LEGEND then
+      [keys[0]] + FilterEncrypted(keys[1..], legend[1..])
+    else
+      FilterEncrypted(keys[1..], legend[1..])
+  }
+
+  // Fail unless the attribute exists, and is a binary terminal
+  function method NeedBinary(data : StructuredDataMap, attr : string): (result: Outcome<Error>)
+  {
+    if attr !in data then
+      Fail(E("The attribute name " + attr + " is required."))
+    else if !data[attr].content.Terminal? then
+      Fail(E(attr + " must be a Terminal."))
+    else if data[attr].content.Terminal.typeId != BYTES_TYPE_ID then
+      Fail(E(attr + " must be a binary Terminal."))
+    else
+      Pass
+  }
+
+  // return the canonical representation of the StructuredData
+  // TODO - implement for real, once we have a spec; but this should still mostly fail at the right times.
+  // second : contins all keys, but some might be encrypted
+  // first : unencrypted versions of anything encrypted in second
+  function method CanonContent (
+    keys : seq<Bytes>,
+    first : map<Bytes, StructuredData>,
+    second : map<Bytes, StructuredData>
+  ) : Bytes
+    requires forall k <- keys :: k in second
+    requires forall k <- first :: first[k].content.Terminal?
+    requires forall k <- second :: second[k].content.Terminal?
+  {
+    if |keys| == 0 then
+      []
+    else if keys[0] in first then
+      GetValue(first[keys[0]]) + CanonContent(keys[1..], first, second)
+    else
+      GetValue(second[keys[0]]) + CanonContent(keys[1..], first, second)
+  }
+
+  // return the footer value for the StructuredData
+  method GetFooter(
+    client: Primitives.AtomicPrimitivesClient,
+    key : Bytes,
+    keys : seq<Bytes>,
+    first : map<Bytes, StructuredData>,
+    second : map<Bytes, StructuredData>,
+    header : Bytes)
+    returns (ret : Result<Bytes, Error>)
+    requires forall k <- keys :: k in second
+    requires forall k <- first :: first[k].content.Terminal?
+    requires forall k <- second :: second[k].content.Terminal?
+  {
+    var data := CanonContent(keys, first, second);
+    var resultR := Digest.Digest(Prim.DigestInput(digestAlgorithm := Prim.SHA_384, message := data));
+    var result :- resultR.MapFailure(e => AwsCryptographyPrimitives(e));
+    return Success(result);
+  }
+
   method EncryptStructure(config: InternalConfig, input: EncryptStructureInput)
     returns (output: Result<EncryptStructureOutput, Error>)
   {
@@ -61,6 +152,7 @@ module AwsCryptographyStructuredEncryptionOperations refines AbstractAwsCryptogr
     );
     var matOutput :- matR.MapFailure(e => AwsCryptographyMaterialProviders(e));
     var mat := matOutput.encryptionMaterials;
+    :- Need(mat.plaintextDataKey.Some?, E("Encryption material has no key"));
 
     //= specification/structured-encryption/header.md#message-id
     //# Implementations MUST generate a fresh 256-bit random MessageID, from a cryptographically secure source, for each record encrypted.
@@ -68,74 +160,56 @@ module AwsCryptographyStructuredEncryptionOperations refines AbstractAwsCryptogr
     var msgID :- randBytes.MapFailure(e => Error.AwsCryptographyPrimitives(e));
     var head :- Header.Create(input.tableName, input.cryptoSchema, msgID, mat.encryptionContext, mat.encryptedDataKeys);
 
-    // TODO: Currently implemented with "fake" encryption for ddb items.
-    // For each attribute that should be encrypted:
-    // - Concatenate typeId and value
-    // - Base64 encode
-    // - Concatenate THIS_IS_NOT_ENCRYPTED and output of the above
-    // - Create a new 'Terminal' with typeId 0x0001 (to be interpreted as string in DDB)
-    //   and value of the output of the above
-    :- Need(input.plaintextStructure.content.DataMap?
-        && input.cryptoSchema.content.SchemaMap?, StructuredEncryptionException(
-      message := "Unexpected Structured Data Item. Currently only implemented to accept DDB Items."
-    ));
+    :- Need(input.plaintextStructure.content.DataMap?, E("Input struture must be a DataMap"));
+    :- Need(input.cryptoSchema.content.SchemaMap?, E("Input Crypto Schema must be a SchemaMap"));
     
-    // Iterate through presumed DDB Item's attributes to perform "fake" encryption
     var cryptoSchema := input.cryptoSchema.content.SchemaMap;
-    var ddbItem := input.plaintextStructure.content.DataMap;
-    var attributeValues := map[];
-    while cryptoSchema.Keys != {}
-    {
-      var attributeName :| attributeName in cryptoSchema;
-      :- Need(cryptoSchema[attributeName].content.Action?
-        && attributeName in ddbItem
-        && ddbItem[attributeName].content.Terminal?, StructuredEncryptionException(
-        message := "Unexpected Structured Data Item. Currently only implemented to accept DDB Items."
-      ));
-      if (cryptoSchema[attributeName].content.Action == CryptoAction.ENCRYPT_AND_SIGN) {
-        var attributeValue := ddbItem[attributeName].content.Terminal;
-        var concatValue := attributeValue.typeId + attributeValue.value;
-        var base64Value := Base64.Encode(concatValue);
-        var base64ValueAsBytes := UTF8.EncodeAscii(base64Value);
-        var finalValue := THIS_IS_NOT_ENCRYPTED + base64ValueAsBytes;
-        var transformedAttribute := StructuredData(
-          content := StructuredDataContent.Terminal(
-            Terminal := StructuredDataTerminal(
-              typeId := DDB_STRING_TYPE_ID,
-              value := finalValue
-            )
-          ),
-          attributes := None
-        );
-        attributeValues := attributeValues[attributeName:=transformedAttribute];
-      } else {
-        // passthrough
-        attributeValues := attributeValues[attributeName:=ddbItem[attributeName]];
-      }
+    :- Need(CryptoSchemaMapIsFlat(cryptoSchema), E("Schema must be flat."));
 
-      cryptoSchema := cryptoSchema - {attributeName};
-    }
-    var headerSerialized :- Header.Serialize(config.primatives, head);
-    var headerString := Base64.Encode(headerSerialized);
-    var headerBytes := UTF8.EncodeAscii(headerString);
-    var headerAttribute := StructuredData(
-      content := StructuredDataContent.Terminal(
-        Terminal := StructuredDataTerminal(
-          typeId := BYTES_TYPE_ID,
-          value := headerBytes
-        )
-      ),
-      attributes := None
-    );
-    attributeValues := attributeValues["aws_ddb_head" := headerAttribute];
+    var plainRecord := input.plaintextStructure.content.DataMap;
+    :- Need(DataMapIsFlat(plainRecord), E("Input DataMap must be flat."));
+    :- Need(HeaderField !in plainRecord, E("The attribute name " + HeaderField + " is reserved."));
+    :- Need(FooterField !in plainRecord, E("The attribute name " + FooterField + " is reserved."));
+    :- Need(plainRecord.Keys == cryptoSchema.Keys, E("Schema must exactly match record"));
+    :- Need(ValidString(input.tableName), E("Bad Table Name"));
+    Paths.SimpleCanonUnique(input.tableName);
+    var canonSchema : map<Bytes, CryptoSchema> := map k | k in cryptoSchema.Keys :: Paths.SimpleCanon(input.tableName, k) := cryptoSchema[k];
+    var canonRecord : map<Bytes, StructuredData> := map k | k in plainRecord.Keys :: Paths.SimpleCanon(input.tableName, k) := plainRecord[k];
+    var keys := Sets.ComputeSetToOrderedSequence2(canonRecord.Keys, Header.ByteLess);
+    assert forall k <- keys :: k in canonRecord;
+    :- Need(forall k <- canonRecord :: canonRecord[k].content.Terminal?, E("Internal Error"));
+    :- Need(forall k <- canonSchema :: canonSchema[k].content.Action?, E("Internal Error"));
 
+    var signedKeys := FilterSchema(keys, canonSchema, a => a != DO_NOTHING);
+    var encryptedKeys := FilterSchema(keys, canonSchema, a => a == ENCRYPT_AND_SIGN);    
+    :- Need(|encryptedKeys| < (UINT32_LIMIT / 3), E("Too many keys"));
+
+    var encryptedItems :- Crypt.Crypt(Crypt.Encrypt, config.primatives, mat.plaintextDataKey.value, head, encryptedKeys, canonRecord);
+    :- Need(|mat.plaintextDataKey.value| == 32, E("Key Wrong Size"));
+    var commitKey := Crypt.GetCommitKey(mat.plaintextDataKey.value, head.msgID);
+    var headerSerialized :- Header.Serialize(config.primatives, commitKey, head);
+    var headerAttribute := ValueToData(headerSerialized, BYTES_TYPE_ID);
+
+    var footer :- GetFooter(config.primatives, mat.plaintextDataKey.value, signedKeys, map[], canonRecord, headerSerialized);
+    var footerAttribute := ValueToData(footer, BYTES_TYPE_ID);
+
+    var result : map<string, StructuredData> := map k | k in plainRecord.Keys :: k :=
+      var c := Paths.SimpleCanon(input.tableName, k);
+      if c in encryptedItems then
+        encryptedItems[c]
+      else
+        plainRecord[k];
+
+    result := result[HeaderField := headerAttribute];
+    result := result[FooterField := footerAttribute];
+    
     var encryptOutput := EncryptStructureOutput(encryptedStructure := StructuredData(
       content := StructuredDataContent.DataMap(
-        DataMap := attributeValues
+        DataMap := result
       ),
       attributes := None
     ));
-    output := Success(encryptOutput);
+    return Success(encryptOutput);
   }
 
   predicate DecryptStructureEnsuresPublicly(
@@ -147,80 +221,81 @@ module AwsCryptographyStructuredEncryptionOperations refines AbstractAwsCryptogr
     && (output.Success? && input.encryptedStructure.content.Terminal? ==> output.value.plaintextStructure.content.Terminal?)
   }
   
-  function method E(message : string) : Error {
-    StructuredEncryptionException(message := message)
-  }
-
   method DecryptStructure(config: InternalConfig, input: DecryptStructureInput)
       returns (output: Result<DecryptStructureOutput, Error>)
   {
-    // TODO: Currently implemented with "fake" decryption for ddb itmes. This is currently brittle,
-    // but for now is useful to demonstrate that the attribute actions are being properly piped
-    // through the system.
-    :- Need(input.encryptedStructure.content.DataMap?, E("Unexpected Structured Data Item. Currently only implemented to accept DDB Items."));
-    
-    // Iterate through presumed DDB Item's attributes to perform "fake" encryption
-    var cryptoSchema := input.encryptedStructure.content.DataMap;
-    :- Need("aws_ddb_head" in cryptoSchema, E("aws_ddb_head field absent"));
-    var headerAttribute := cryptoSchema["aws_ddb_head"];
-    :- Need(headerAttribute.content.Terminal?, E("aws_ddb_head must be a Terminal"));
-    var headerBytes := headerAttribute.content.Terminal.value;
-    var headerStringR := UTF8.Decode(headerBytes);
-    var headerString :- headerStringR.MapFailure(e => E(e));
-    var headerSerializedR := Base64.Decode(headerString);
-    var headerSerialized :- headerSerializedR.MapFailure(e => E(e));
-    var head :- Header.Deserialize(config.primatives, headerSerialized);
+    :- Need(input.authenticateSchema.content.SchemaMap?, E("Authenticate Schema must be a SchemaMap"));
+    var authSchema := input.authenticateSchema.content.SchemaMap;
+    :- Need(AuthSchemaIsFlat(authSchema), E("Schema must be flat."));
 
-    var attributeValues := map[];
-    while cryptoSchema.Keys != {}
-    {
-      var attributeName :| attributeName in cryptoSchema;
-      :- Need(cryptoSchema[attributeName].content.Terminal?, E("Unexpected Structured Data Item. Currently only implemented to accept DDB Items."));
-      var attributeValue := cryptoSchema[attributeName].content.Terminal;
-      // Since we are not storing the cryptoSchema that was used on encrypt,
-      // for our "fake" approach simply look for attributes that appear to be
-      // "fake" encrypted. Anyone testing integration with this fake encryption
-      // MUST NOT use the value "THIS_IS_NOT_ENCRYPTED" in their data set.
-      if (attributeValue.typeId == DDB_STRING_TYPE_ID
-          && |attributeValue.value| >= |THIS_IS_NOT_ENCRYPTED|
-          && attributeValue.value[..|THIS_IS_NOT_ENCRYPTED|] == THIS_IS_NOT_ENCRYPTED) {
-        // To "fake" decrypt:
-        // - String "THIS_IS_NOT_ENCRYPTED"
-        // - Base64 Decode the rest
-        // - Grab the first two bytes as typeId, the rest are the serialized value
-        var base64Value := attributeValue.value[|THIS_IS_NOT_ENCRYPTED|..];
-        var base64AsChar :- UTF8.Decode(base64Value)
-            .MapFailure(e => Types.StructuredEncryptionException( message := e ));
-        var concatValue :- Base64.Decode(base64AsChar)
-            .MapFailure(e => Types.StructuredEncryptionException( message := e ));
-        :- Need(|concatValue| >= 2, StructuredEncryptionException(
-          message := "Invalid 'fake' encryption: Missing typeId"
-        ));
-        var originalTypeId := concatValue[..2];
-        var originalValue := concatValue[2..];
-        var untransformedAttribute := StructuredData(
-          content := StructuredDataContent.Terminal(
-            Terminal := StructuredDataTerminal(
-              typeId := originalTypeId,
-              value := originalValue
-            )
-          ),
-          attributes := None
-        );
-        attributeValues := attributeValues[attributeName:=untransformedAttribute];
-      } else {
-        // else it is not "fake" encrypted, so pass through
-        attributeValues := attributeValues[attributeName:=cryptoSchema[attributeName]];
-      }
+    :- Need(input.encryptedStructure.content.DataMap?, E("Input struture must be a DataMap"));
+    var encRecord := input.encryptedStructure.content.DataMap;
+    :- Need(DataMapIsFlat(encRecord), E("Input DataMap must be flat."));
+    :- Need(authSchema.Keys == encRecord.Keys, E("Authenticate schema must match encrypted structure exactly."));
+    :- NeedBinary(encRecord, HeaderField);
+    :- NeedBinary(encRecord, FooterField);
 
-      cryptoSchema := cryptoSchema - {attributeName};
+    var headerSerialized := encRecord[HeaderField].content.Terminal.value;
+    var footerSerialized := encRecord[FooterField].content.Terminal.value;
+    var head :- Header.PartialDeserialize(headerSerialized);
+
+    var matR := input.cmm.DecryptMaterials(
+      CMP.DecryptMaterialsInput (
+        algorithmSuiteId := Defaults.GetAlgorithmSuiteForCommitmentPolicy(CMP.CommitmentPolicy.ESDK(CMP.REQUIRE_ENCRYPT_REQUIRE_DECRYPT)),
+        commitmentPolicy := CMP.CommitmentPolicy.ESDK(CMP.REQUIRE_ENCRYPT_REQUIRE_DECRYPT),
+        encryptedDataKeys := head.dataKeys,
+        encryptionContext := head.encContext
+      )
+    );
+
+    var matOutput :- matR.MapFailure(e => AwsCryptographyMaterialProviders(e));
+    var mat := matOutput.decryptionMaterials;
+    :- Need(mat.plaintextDataKey.Some?, E("Encryption material has no key"));
+
+    :- Need(|mat.plaintextDataKey.value| == 32, E("Key Wrong Size"));
+    var commitKey := Crypt.GetCommitKey(mat.plaintextDataKey.value, head.msgID);
+    var ok :- head.check(config.primatives, commitKey, headerSerialized);
+
+    :- Need(ValidString(input.tableName), E("Bad Table Name"));
+    Paths.SimpleCanonUnique(input.tableName);
+
+    var canonSchema : map<Bytes, AuthenticateSchema> := map k <- authSchema :: Paths.SimpleCanon(input.tableName, k) := authSchema[k];
+    var canonRecord : map<Bytes, StructuredData> := map k <- encRecord :: Paths.SimpleCanon(input.tableName, k) := encRecord[k];
+    var keys := Sets.ComputeSetToOrderedSequence2(canonRecord.Keys, Header.ByteLess);
+    :- Need(forall k <- canonRecord :: canonRecord[k].content.Terminal?, E("Internal Error"));
+    :- Need(forall k <- canonSchema :: canonSchema[k].content.Action?, E("Internal Error"));
+
+    var signedKeys := FilterAuth(keys, canonSchema, SIGN);
+    if |head.legend| < |signedKeys| {
+      return Failure(E("Schema changed : something that was unsigned is now signed."));
     }
+    if |head.legend| > |signedKeys| {
+      return Failure(E("Schema changed : something that was signed is now unsigned."));
+    }
+    assert |head.legend| == |signedKeys|;
+
+    var encryptedKeys := FilterEncrypted(signedKeys, head.legend);
+    :- Need(|encryptedKeys| < (UINT32_LIMIT / 3), E("Too many keys"));
+
+    var decryptedItems :- Crypt.Crypt(Crypt.Decrypt, config.primatives, mat.plaintextDataKey.value, head, encryptedKeys, canonRecord);
+
+    var result : map<string, StructuredData> := map k | k in encRecord.Keys :: k :=
+      var c := Paths.SimpleCanon(input.tableName, k);
+      if c in decryptedItems then
+        decryptedItems[c]
+      else
+        encRecord[k];
+
+    var footer :- GetFooter(config.primatives, mat.plaintextDataKey.value, signedKeys, decryptedItems, canonRecord, headerSerialized);
+    :- Need(footer == footerSerialized, E("Footer mismatch."));
+
     var decryptOutput := DecryptStructureOutput(plaintextStructure := StructuredData(
       content := StructuredDataContent.DataMap(
-        DataMap := attributeValues
+        DataMap := result - {HeaderField, FooterField}
       ),
       attributes := None
     ));
+
     output := Success(decryptOutput);
   }
 }
