StructuredEncryption/src/Crypt.dfy
@@ -1,0 +1,191 @@
+// Copyright Amazon.com Inc. or its affiliates. All Rights Reserved.
+// SPDX-License-Identifier: Apache-2.0
+
+include "../Model/AwsCryptographyStructuredEncryptionTypes.dfy"
+include "Header.dfy"
+include "Util.dfy"
+
+module StructuredEncryptionCrypt {
+  import opened Wrappers
+  import opened StandardLibrary
+  import opened StandardLibrary.UInt
+  import opened AwsCryptographyStructuredEncryptionTypes
+  import opened StructuredEncryptionUtil
+
+  import CMP = AwsCryptographyMaterialProvidersTypes
+  import Prim = AwsCryptographyPrimitivesTypes
+  import Aws.Cryptography.Primitives
+  import UTF8
+  import Header = StructuredEncryptionHeader
+  import HKDF
+
+  const KeySize := 32 // 256 bits, for 256-bit AES keys
+  const NonceSize := 12 // 96 bits, per AES-GCM nonces
+  const AuthTagSize := 16
+
+  // TODO - an extern that actually does AES CTR
+  function method aes256ctr(length : nat, key : Bytes, nonce : Bytes)
+    : (ret : Bytes)
+    ensures |ret| == length
+  {
+    seq(length, i => (i % 256) as uint8)
+  }
+
+  function method FieldKey(HKDFOutput : Bytes, offset : uint32)
+    : (ret : Bytes)
+    requires |HKDFOutput| == KeySize
+    ensures |ret| == KeySize+NonceSize
+  {
+    (HKDFOutput+HKDFOutput)[..44] // good enough for testing
+    //aes256ctr(KeySize+NonceSize, HKDFOutput, FieldKeyNonce(offset * 3))
+  }
+
+  function method FieldKeyNonce(offset : uint32)
+    : (ret : Bytes)
+    ensures |ret| == 16
+    {
+        UTF8.EncodeAscii("Truss")
+      + [0]
+      + UTF8.EncodeAscii("Field")
+      + [(KeySize+NonceSize) as uint8] // length
+      + UInt32ToSeq(offset)
+    }
+    
+  // the underscore is not present in the AWS Encryption SDK's constants
+  const LABEL_COMMITMENT_KEY := UTF8.EncodeAscii("TRUSS_COMMIT_KEY")
+  const LABEL_ENCRYPTION_KEY := UTF8.EncodeAscii("TRUSS_DERIVE_KEY")
+  
+  // suitable for header field
+  method GetCommitKey(key : CMP.Secret, msgID : Bytes) returns (ret : Bytes)
+    requires |msgID| == 32
+    requires |key| == KeySize
+  {
+    ret := HKDF.Hkdf(
+      Prim.SHA_512, 
+      None, // salt
+      key, // ikm
+      LABEL_COMMITMENT_KEY + msgID, // info
+      KeySize // length
+    );
+  }
+
+  datatype EncryptionSelector = Encrypt | Decrypt
+
+  // Encrypt or Decrypt a StructuredDataMap
+  method Crypt(
+    mode : EncryptionSelector,
+    client: Primitives.AtomicPrimitivesClient,
+    key : Bytes,
+    head : Header.PartialHeader,
+    keys : seq<Bytes>,
+    data : map<Bytes, StructuredData>)
+    returns (ret : Result<map<Bytes, StructuredData>, Error>)
+    requires forall k <- keys :: k in data
+    requires |keys| < (UINT32_LIMIT / 3)
+    requires forall k <- data :: data[k].content.Terminal?
+    ensures ret.Success? ==> forall k <- ret.value :: ret.value[k].content.Terminal?
+
+    modifies client.Modifies
+    requires client.ValidState()
+    ensures client.ValidState()
+  {
+    :- Need(|key| < INT32_MAX_LIMIT, E("key too long"));
+
+    var FieldRootKey := HKDF.Hkdf(
+      Prim.SHA_512, 
+      None, // salt
+      key, // ikm
+      LABEL_ENCRYPTION_KEY + head.msgID, // info
+      KeySize // length
+    );
+    var result := CryptList(mode, client, FieldRootKey, 0, keys, data, map[]);
+    return result;
+  }
+
+  // Encrypt or Decrypt each entry in keys, putting results in output
+  method {:tailrecursion} CryptList(
+    mode : EncryptionSelector,
+    client: Primitives.AtomicPrimitivesClient,
+    FieldRootKey : Bytes,
+    offset : uint32,
+    keys : seq<Bytes>,
+    input : map<Bytes, StructuredData>,
+    output : map<Bytes, StructuredData>
+  )
+    returns (ret : Result<map<Bytes, StructuredData>, Error>)
+    requires forall k <- keys :: k in input
+    requires |keys| * 3 + (offset as nat) < UINT32_LIMIT
+    requires |FieldRootKey| == KeySize
+    requires forall k <- input :: input[k].content.Terminal?
+    requires forall k <- output :: output[k].content.Terminal?
+    ensures ret.Success? ==> forall k <- ret.value :: ret.value[k].content.Terminal?
+    decreases |keys|
+
+    modifies client.Modifies
+    requires client.ValidState()
+    ensures client.ValidState()
+  {
+    if |keys| == 0 {
+      return Success(output);
+    }
+    var data :- CryptOne(mode, client, FieldRootKey, offset, input[keys[0]]);
+    var result := CryptList(mode, client, FieldRootKey, offset+1, keys[1..], input, output[keys[0] := data]);
+    return result;
+  }
+
+  // Encrypt or Decrypt a single Terminal
+  method CryptOne(
+    mode : EncryptionSelector,
+    client: Primitives.AtomicPrimitivesClient,
+    FieldRootKey : Bytes,
+    offset : uint32,
+    data : StructuredData
+  )
+    returns (ret : Result<StructuredData, Error>)
+    requires |FieldRootKey| == KeySize
+    requires data.content.Terminal?
+    ensures ret.Success? ==> ret.value.content.Terminal?
+
+    modifies client.Modifies
+    requires client.ValidState()
+    ensures client.ValidState()
+  {
+    var dataKey := FieldKey(FieldRootKey, offset);
+    var encryptionKey := dataKey[0..KeySize];
+    var nonce := dataKey[KeySize..];
+
+    // TODO - algorithm suite
+    var encAlg := Prim.AES_GCM(keyLength := KeySize as Prim.SymmetricKeyLength, tagLength := AuthTagSize as Prim.Uint8Bits, ivLength := NonceSize as Prim.Uint8Bits);
+    var value := data.content.Terminal.value;
+    if mode == Encrypt {
+      var encInput := Prim.AESEncryptInput(
+        encAlg := encAlg,
+        iv := nonce,
+        key := encryptionKey,
+        msg := data.content.Terminal.typeId + value,
+        aad := [] // encryption context
+      );
+
+      var encOutR := client.AESEncrypt(encInput);
+      var encOut :- encOutR.MapFailure(e => AwsCryptographyPrimitives(e));
+      return Success(ValueToData(encOut.cipherText + encOut.authTag, [0xff, 0xff]));
+    } else {
+      :- Need(AuthTagSize <= |value|, E("cipherTxt too short."));
+      var decInput := Prim.AESDecryptInput(
+        encAlg := encAlg,
+        iv := nonce,
+        key := encryptionKey,
+        cipherTxt := value[..|value| - AuthTagSize],
+        aad := [], // enc context
+        authTag := value[|value|-AuthTagSize..]
+      );
+
+      var decOutR := client.AESDecrypt(decInput);
+      var decOut :- decOutR.MapFailure(e => AwsCryptographyPrimitives(e));
+      :- Need(2 <= |decOut|, E("Too little data."));
+      return Success(ValueToData(decOut[2..], decOut[..2]));
+    }
+  }
+
+
+}
