StructuredEncryption/src/Util.dfy
@@ -1,0 +1,82 @@
+// Copyright Amazon.com Inc. or its affiliates. All Rights Reserved.
+// SPDX-License-Identifier: Apache-2.0
+
+include "../Model/AwsCryptographyStructuredEncryptionTypes.dfy"
+
+module StructuredEncryptionUtil {
+  import opened AwsCryptographyStructuredEncryptionTypes
+  import opened Wrappers
+  import opened StandardLibrary
+  import opened StandardLibrary.UInt
+  import UTF8
+
+  // These two should be part of the DDB layer, and passed in somehow
+  // Or maybe part of AwsCryptographyStructuredEncryptionOperations.Config?
+  const HeaderField := "aws_ddb_head"
+  const FooterField := "aws_ddb_foot"
+
+  const BYTES_TYPE_ID : seq<uint8> := [0xFF, 0xFF];
+
+  type Bytes = seq<uint8>
+  type GoodString = x : string | ValidString(x)
+  predicate method ValidString(x : string)
+  {
+    && |x| <  UINT64_LIMIT
+    && UTF8.Encode(x).Success?
+  }
+
+  // string to Error
+  function method E(s : string) : Error {
+    StructuredEncryptionException(message := s)
+  }
+
+  // Is the CryptoSchemaMap flat, i.e., does it contain only Actions?
+  function method CryptoSchemaMapIsFlat(data : CryptoSchemaMap) : (ret : bool)
+    ensures ret ==> (forall v <- data.Values :: v.content.Action?)
+  {
+    forall v <- data.Values :: v.content.Action? 
+  }
+
+  // Schema must contain only Actions
+  function method AuthSchemaIsFlat(data : AuthenticateSchemaMap) : (ret : bool)
+    ensures ret ==> (forall v <- data.Values :: v.content.Action?)
+  {
+    forall v <- data.Values :: v.content.Action? 
+  }
+
+  // Map must contain only Terminals
+  function method DataMapIsFlat(data : StructuredDataMap) : (ret : bool)
+    ensures ret ==> (forall v <- data.Values :: v.content.Terminal?)
+  {
+    forall v <- data.Values :: v.content.Terminal? 
+  }
+
+  // attibute is "authorized", a.k.a. included in the signature
+  predicate method IsAuthAttr(x : CryptoAction)
+  {
+    x.ENCRYPT_AND_SIGN? || x.SIGN_ONLY?
+  }
+
+  // wrap a value in a StructuredData
+  function method ValueToData(value : Bytes, typeId : Bytes)
+    : StructuredData
+    requires IsValid_TerminalTypeId(typeId)
+  {
+    StructuredData(
+      content := StructuredDataContent.Terminal(
+        Terminal := StructuredDataTerminal(
+          typeId := typeId,
+          value := value
+        )
+      ),
+      attributes := None
+    )
+  }
+
+  // extract a value from a StructuredData
+  function method GetValue(data : StructuredData) : Bytes
+    requires data.content.Terminal?
+  {
+    data.content.Terminal.value
+  }
+}
